New structure for parser_kind. Simplified integer proofs

src/lowparse/LowParse.SLow.Int.fst
@@ -1,36 +1,33 @@
 module LowParse.SLow.Int
-include LowParse.SLow.Int.Proof
+include LowParse.Spec.Int
+include LowParse.SLow.Combinators
 
 module Seq = FStar.Seq
-module E = LowParse.BigEndian
+module E = LowParse.BigEndianImpl
 module U8  = FStar.UInt8
 module U16 = FStar.UInt16
 module U32 = FStar.UInt32
 module B32 = FStar.Bytes
-module Cast = FStar.Int.Cast
 
 inline_for_extraction
 let serialize32_u8
 : serializer32 serialize_u8
 = (fun (input: U8.t) ->
-    serialize32_u8_correct input;
-    (serialize32_u8' input <: (res: bytes32 { serializer32_correct #_ #_ #parse_u8 serialize_u8 input res } )))
+    let b = B32.create 1ul input in
+    b32_reveal_create 1ul input;
+    (b <: (res: bytes32 { serializer32_correct #_ #_ #parse_u8 serialize_u8 input res } )))
 
 inline_for_extraction
 let serialize32_u16 : serializer32 #_ #_ #parse_u16 serialize_u16 =
-  (fun (input: U16.t) -> ((
-    let b = B32.create 2ul 42uy in
-    serialize32_u16_correct b input;
-    serialize32_u16' b input
-  ) <: (res: B32.bytes { serializer32_correct #_ #_ #parse_u16 serialize_u16 input res } )))
+  (fun (input: U16.t) ->
+    let b = E.n_to_be_impl _ _ E.u16 2ul input () in
+    (b <: (res: B32.bytes { serializer32_correct #_ #_ #parse_u16 serialize_u16 input res } )))
 
 inline_for_extraction
 let serialize32_u32 : serializer32 #_ #_ #parse_u32 serialize_u32 =
-  (fun (input: U32.t) -> ((
-    let b = B32.create 4ul 42uy in
-    serialize32_u32_correct b input;
-    serialize32_u32' b input
-  ) <: (res: B32.bytes { serializer32_correct #_ #_ #parse_u32 serialize_u32 input res } )))
+  (fun (input: U32.t) ->
+    let b = E.n_to_be_impl _ _ E.u32 4ul input () in
+    (b <: (res: B32.bytes { serializer32_correct #_ #_ #parse_u32 serialize_u32 input res } )))
 
 inline_for_extraction
 let parse32_u16 : parser32 parse_u16 =
@@ -40,8 +37,8 @@ let parse32_u16 : parser32 parse_u16 =
       decode_u16
       ()
       (fun (input: B32.lbytes 2) ->
-        decode32_u16_correct input;
-        (decode32_u16' input <: (res: U16.t { res == decode_u16 (B32.reveal input) } )))
+        let res = E.be_to_n_impl _ _ E.u16 input in
+        (res <: (res: U16.t { res == decode_u16 (B32.reveal input) } )))
 
 inline_for_extraction
 let parse32_u32 : parser32 parse_u32 =
@@ -51,13 +48,12 @@ let parse32_u32 : parser32 parse_u32 =
       decode_u32
       ()
       (fun (input: B32.lbytes 4) ->
-        decode32_u32_correct input;
-        (decode32_u32' input <: (res: U32.t { res == decode_u32 (B32.reveal input) } )))
-
-#set-options "--z3rlimit 128"
+        let res = E.be_to_n_impl _ _ E.u32 input in
+        (res <: (res: U32.t { res == decode_u32 (B32.reveal input) } )))
 
 inline_for_extraction
 let parse32_u8 : parser32 parse_u8 =
+  decode_u8_injective ();
   make_total_constant_size_parser32 1 1ul
     decode_u8
     ()
