src/lowparse/LowParse.SLow.VLData.fst
@@ -1,139 +1,40 @@
 module LowParse.SLow.VLData
-include LowParse.SLow.VLData.Proof
+include LowParse.Spec.VLData
+include LowParse.SLow.FLData
 
 module Seq = FStar.Seq
-module U8 = FStar.UInt8
-module U16 = FStar.UInt16
 module U32 = FStar.UInt32
-module E = LowParse.BigEndian
-module Cast = FStar.Int.Cast
+module E = LowParse.BigEndianImpl
 module B32 = FStar.Bytes
-
-inline_for_extraction
-let serialize32_bounded_integer_1 : serializer32 (serialize_bounded_integer 1) =
-  (fun (input: bounded_integer 1) -> ((
-    let b = B32.create 1ul 42uy in
-    [@inline_let]
-    let _ = serialize32_bounded_integer_1_correct b input in
-    serialize32_bounded_integer_1' b input
-  ) <: (res: B32.bytes { serializer32_correct (serialize_bounded_integer 1) input res } )))
-
-inline_for_extraction
-let serialize32_bounded_integer_2 : serializer32 (serialize_bounded_integer 2) =
-  (fun (input: bounded_integer 2) -> ((
-    let b = B32.create 2ul 42uy in
-    [@inline_let]
-    let _ = serialize32_bounded_integer_2_correct b input in
-    serialize32_bounded_integer_2' b input
-  ) <: (res: B32.bytes { serializer32_correct (serialize_bounded_integer 2) input res } )))
-
-inline_for_extraction
-let serialize32_bounded_integer_3 : serializer32 (serialize_bounded_integer 3) =
-  (fun (input: bounded_integer 3) -> ((
-    let b = B32.create 3ul 42uy in
-    [@inline_let]
-    let _ = serialize32_bounded_integer_3_correct b input in
-    serialize32_bounded_integer_3' b input
-  ) <: (res: B32.bytes { serializer32_correct (serialize_bounded_integer 3) input res } )))
-
-inline_for_extraction
-let serialize32_bounded_integer_4 : serializer32 (serialize_bounded_integer 4) =
-  serialize32_u32
-
-inline_for_extraction
-let serialize_bounded_integer_conv
-  (sz sz' : integer_size)
-  (s32: serializer32 (serialize_bounded_integer sz))
-: Pure (serializer32 (serialize_bounded_integer sz'))
-  (requires (sz == sz'))
-  (ensures (fun _ -> True))
-= s32
 
 inline_for_extraction
 let serialize32_bounded_integer
   (sz: integer_size)
 : Tot (serializer32 (serialize_bounded_integer sz))
-= match sz with
-  | 1 -> serialize_bounded_integer_conv 1 sz serialize32_bounded_integer_1
-  | 2 -> serialize_bounded_integer_conv 2 sz serialize32_bounded_integer_2
-  | 3 -> serialize_bounded_integer_conv 3 sz serialize32_bounded_integer_3
-  | 4 -> serialize_bounded_integer_conv 4 sz serialize32_bounded_integer_4
-
-inline_for_extraction
-let decode32_bounded_integer_1
- (b: B32.lbytes 1)
-: Tot (y: bounded_integer 1 { y == decode_bounded_integer 1 (B32.reveal b) } )
 = [@inline_let]
-  let r = decode32_bounded_integer_1' b in
-  [@inline_let]
-  let _ = decode32_bounded_integer_1_correct b in
-  (r <: (r: bounded_integer 1 { r == decode_bounded_integer 1 (B32.reveal b) } ))
-
-inline_for_extraction
-let parse32_bounded_integer_1 : parser32 (parse_bounded_integer 1) =
-  [@inline_let]
-  let _ = decode_bounded_integer_injective 1 in
-  make_total_constant_size_parser32 1 1ul
-    (decode_bounded_integer 1)
-    ()
-    (decode32_bounded_integer_1)
-
-inline_for_extraction
-let parse32_bounded_integer_2 : parser32 (parse_bounded_integer 2) =
-  fun (input: bytes32) -> (
-    [@inline_let]
-    let res = parse32_synth parse_u16 synth_bounded_integer_2 (fun (x: U16.t) -> (Cast.uint16_to_uint32 x <: (y: bounded_integer 2 { y == synth_bounded_integer_2 x } ))) parse32_u16 () input in
-    parse_bounded_integer_2_spec ();
-    (res <: (res: option (bounded_integer 2 * U32.t) { parser32_correct (parse_bounded_integer 2) input res} ))
+  let sz32 = U32.uint_to_t sz in
+  (fun (input: bounded_integer sz) ->
+    let b = E.n_to_be_impl _ _ E.u32 sz32 input () in
+    (b <: (res: B32.bytes { serializer32_correct (serialize_bounded_integer sz) input res } ))
   )
 
 inline_for_extraction
-let decode32_bounded_integer_3
- (b: B32.lbytes 3)
-: Tot (y: bounded_integer 3 { y == decode_bounded_integer 3 (B32.reveal b) } )
-= [@inline_let]
-  let r = decode32_bounded_integer_3' b in
+let decode32_bounded_integer
+  (sz: integer_size)
+  (b: B32.lbytes sz)
+: Tot (y: bounded_integer sz { y == decode_bounded_integer sz (B32.reveal b) } )
+= let r = E.be_to_n_impl _ _ E.u32 b in
+  E.lemma_be_to_n_is_bounded (B32.reveal b);
+  (r <: (r: bounded_integer sz { r == decode_bounded_integer sz (B32.reveal b) } ))
+
+inline_for_extraction
+let parse32_bounded_integer (sz: integer_size) : Tot (parser32 (parse_bounded_integer sz)) =
   [@inline_let]
-  let _ = decode32_bounded_integer_3_correct b in
-  (r <: (r: bounded_integer 3 { r == decode_bounded_integer 3 (B32.reveal b) } ))
-
-inline_for_extraction
-let parse32_bounded_integer_3 : parser32 (parse_bounded_integer 3) =
-  decode_bounded_integer_injective 3;
-  make_total_constant_size_parser32 3 3ul
-    (decode_bounded_integer 3)
+  let _ = decode_bounded_integer_injective sz in
+  make_total_constant_size_parser32 sz (U32.uint_to_t sz)
+    (decode_bounded_integer sz)
     ()
-    (decode32_bounded_integer_3)
-
-inline_for_extraction
-let parse32_bounded_integer_4 : parser32 (parse_bounded_integer 4) =
-  fun (input: bytes32) -> (
-    [@inline_let]
-    let res = parse32_synth parse_u32 synth_bounded_integer_4 (fun (x: U32.t) -> (x <: (y: bounded_integer 4 { y == synth_bounded_integer_4 x } ))) parse32_u32 () input in
-    parse_bounded_integer_4_spec ();
-    (res <: (res: option (bounded_integer 4 * U32.t) { parser32_correct (parse_bounded_integer 4) input res} ))
-  )
-
-inline_for_extraction
-let parse_bounded_integer_conv
-  (sz sz' : integer_size)
-  (s32: parser32 (parse_bounded_integer sz))
-: Pure (parser32 (parse_bounded_integer sz'))
-  (requires (sz == sz'))
-  (ensures (fun _ -> True))
-= s32
-
-inline_for_extraction
-let parse32_bounded_integer
-  (i: integer_size)
-: Tot (parser32 (parse_bounded_integer i))
-= [@inline_let]
-  let _ = integer_size_values i in
-  match i with
-  | 1 -> parse_bounded_integer_conv 1 i parse32_bounded_integer_1
-  | 2 -> parse_bounded_integer_conv 2 i parse32_bounded_integer_2
-  | 3 -> parse_bounded_integer_conv 3 i parse32_bounded_integer_3
-  | 4 -> parse_bounded_integer_conv 4 i parse32_bounded_integer_4
+    (decode32_bounded_integer sz)
 
 (* Parsers and serializers for the payload *)
 
