src/lowparse/LowParse.BigEndianImpl.fst
@@ -1,0 +1,270 @@
+module LowParse.BigEndianImpl
+include LowParse.BigEndian
+
+module U = FStar.UInt
+module U8 = FStar.UInt8
+
+noeq
+type uinttype (t: Type0) (n: nat) =
+  | UIntType:
+    (v: (t -> Tot (y: nat { U.fits y n } ))) ->
+    (to_byte: ((x: t) -> Tot (y: U8.t { U8.v y == v x % 256 } ))) ->
+    (from_byte: ((x: U8.t) -> Tot (y: t { v y == U8.v x } ))) ->
+    (zero: t { v zero == 0 } ) ->
+    (v_inj: ((x1: t) -> (x2: t) -> Lemma (requires (v x1 == v x2)) (ensures (x1 == x2)))) ->
+    (add: ((x: t) -> (y: t) -> Pure t (requires (U.fits (v x + v y) n)) (ensures (fun z -> v z == v x + v y)))) ->
+    (mul256: ((x: t) -> Pure t (requires (U.fits (Prims.op_Multiply (v x) 256) n)) (ensures (fun z -> v z == Prims.op_Multiply (v x) 256)))) ->
+    (div256: ((x: t) -> Pure t (requires True) (ensures (fun z -> v z == v x / 256)))) ->
+    uinttype t n
+
+module Seq = FStar.Seq
+module B32 = FStar.Bytes
+module U32 = FStar.UInt32
+module M = LowParse.Math
+module G = FStar.Ghost
+
+#reset-options "--z3rlimit 16"
+
+inline_for_extraction
+let be_to_n_body'
+  (t: Type0)
+  (n: nat)
+  (u: uinttype t n)
+  (s: B32.bytes)
+  (i: U32.t)
+  (accu: t)
+: Pure t
+  (requires (
+    0 < U32.v i /\
+    U32.v i <= B32.length s /\
+    Prims.op_Multiply 8 (B32.length s) <= n /\
+    u.v accu == be_to_n (Seq.slice (B32.reveal s) 0 (B32.length s - U32.v i))
+  ))
+  (ensures (fun accu' ->
+    u.v accu' == be_to_n (Seq.slice (B32.reveal s) 0 (B32.length s - (U32.v i - 1)))
+  ))
+= let sq = G.hide (Seq.slice (B32.reveal s) 0 (B32.length s - U32.v i)) in
+  let sq' = G.hide (Seq.slice (B32.reveal s) 0 (B32.length s - (U32.v i - 1))) in
+  let b = B32.get s (U32.sub (B32.len s) i) in
+  assert (b == Seq.last (G.reveal sq'));
+  assert (Seq.slice (G.reveal sq') 0 (Seq.length (G.reveal sq') - 1) == G.reveal sq);
+  lemma_be_to_n_is_bounded (G.reveal sq);
+  M.pow2_plus (8 `Prims.op_Multiply` Seq.length (G.reveal sq)) 8;
+  assert (u.v accu `Prims.op_Multiply` 256 < pow2 (8 `Prims.op_Multiply` Seq.length (G.reveal sq) + 8));
+  M.pow2_le_compat n (8 `Prims.op_Multiply` Seq.length (G.reveal sq) + 8);
+  assert (u.v accu `Prims.op_Multiply` 256 < pow2 n);
+  let accu256 = u.mul256 accu in
+  let accu' = u.add (u.from_byte b) accu256 in
+  accu'
+
+let be_to_n_inv
+  (t: Type0)
+  (n: nat)
+  (u: uinttype t n)
+  (s: B32.bytes)
+  (continue: bool)
+  (x: U32.t * t)
+: GTot Type0
+= let (i, accu) = x in
+  U32.v i <= B32.length s /\
+  8 `Prims.op_Multiply` B32.length s <= n /\
+  u.v accu == be_to_n (Seq.slice (B32.reveal s) 0 (B32.length s - U32.v i)) /\
+  (continue == false ==> U32.v i == 0)
+
+let be_to_n_measure
+  (t: Type0)
+  (x: U32.t * t)
+: GTot nat
+= let (i, _) = x in
+  U32.v i
+
+inline_for_extraction
+let be_to_n_body
+  (t: Type0)
+  (n: nat)
+  (u: uinttype t n)
+  (s: B32.bytes)
+  (x: U32.t * t)
+: Pure (bool * (U32.t * t))
+  (requires (be_to_n_inv t n u s true x))
+  (ensures (fun (continue, x') ->
+    be_to_n_inv t n u s continue x' /\
+    (continue == true ==>  be_to_n_measure t x' < be_to_n_measure t x)
+  ))
+= let (i, accu) = x in
+  if i = 0ul
+  then (false, x)
+  else
+    let accu' = be_to_n_body' t n u s i accu in
+    let i' = U32.sub i 1ul in
+    (true, (i', accu'))
+
+module CL = C.Loops
+
+inline_for_extraction
+let be_to_n_impl 
+  (t: Type0)
+  (n: nat)
+  (u: uinttype t n)
+  (s: B32.bytes)
+: Pure t
+  (requires (8 `Prims.op_Multiply` B32.length s <= n))
+  (ensures (fun y -> u.v y == be_to_n (B32.reveal s)))
+= let (_, res) =
+    CL.total_while
+      (be_to_n_measure t)
+      (be_to_n_inv t n u s)
+      (be_to_n_body t n u s)
+      (B32.len s, u.zero)
+  in
+  res
+
+inline_for_extraction
+let n_to_be_body'
+  (t: Type0)
+  (n: nat)
+  (u: uinttype t n)
+  (x0: t)
+  (i: U32.t)
+  (x: t)
+  (accu: B32.bytes)
+: Pure B32.bytes
+  (requires (
+    8 `Prims.op_Multiply` B32.length accu <= n /\
+    U32.v i <= B32.length accu /\
+    0 < U32.v i /\
+    u.v x0 < pow2 (8 `Prims.op_Multiply` B32.length accu) /\
+    u.v x < pow2 (8 `Prims.op_Multiply` U32.v i) /\
+    n_to_be (B32.len accu) (u.v x0) == Seq.append (n_to_be i (u.v x)) (Seq.slice (B32.reveal accu) (U32.v i) (B32.length accu))
+  ))
+  (ensures (fun accu' ->
+    B32.length accu' == B32.length accu /\ (
+    let x' = u.div256 x in
+    let i' = U32.sub i 1ul in
+    u.v x' < pow2 (8 `Prims.op_Multiply` U32.v i') /\
+    n_to_be (B32.len accu') (u.v x0) == Seq.append (n_to_be i' (u.v x')) (Seq.slice (B32.reveal accu') (U32.v i') (B32.length accu'))
+  )))
+= let b = u.to_byte x in
+  let i' = U32.sub i 1ul in
+  let accu' = B32.set_byte accu i' b in
+  M.pow2_plus 8 (8 `Prims.op_Multiply` U32.v i');
+  let x' = G.hide (u.div256 x) in
+  assert (u.v (G.reveal x') < pow2 (8 `Prims.op_Multiply` U32.v i'));
+  assert (n_to_be i (u.v x) == Seq.append (n_to_be i' (u.v (G.reveal x'))) (Seq.create 1 b));
+  assert (Seq.slice (B32.reveal accu') (U32.v i) (B32.length accu') == Seq.slice (B32.reveal accu) (U32.v i) (B32.length accu));
+  assert (Seq.slice (B32.reveal accu') (U32.v i') (B32.length accu') `Seq.equal` Seq.append (Seq.create 1 b) (Seq.slice (B32.reveal accu') (U32.v i) (B32.length accu')));
+  Seq.append_assoc (n_to_be i' (u.v (G.reveal x'))) (Seq.create 1 b) (Seq.slice (B32.reveal accu') (U32.v i) (B32.length accu'));
+  accu'
+
+let n_to_be_inv
+  (t: Type0)
+  (n: nat)
+  (u: uinttype t n)
+  (len: U32.t)
+  (x0: t)
+  (continue: bool)
+  (y: U32.t * t * B32.bytes)
+: GTot Type0
+= let (i, x, accu) = y in
+    U32.v len == B32.length accu /\
+    8 `Prims.op_Multiply` B32.length accu <= n /\
+    U32.v i <= B32.length accu /\
+    u.v x0 < pow2 (8 `Prims.op_Multiply` B32.length accu) /\
+    u.v x < pow2 (8 `Prims.op_Multiply` U32.v i) /\
+    n_to_be (B32.len accu) (u.v x0) == Seq.append (n_to_be i (u.v x)) (Seq.slice (B32.reveal accu) (U32.v i) (B32.length accu)) /\
+    (continue == false ==> U32.v i == 0)
+
+let n_to_be_measure
+  (t: Type0)
+  (y: U32.t * t * B32.bytes)
+: GTot nat
+= let (i, _, _) = y in
+  U32.v i
+
+inline_for_extraction
+let n_to_be_body
+  (t: Type0)
+  (n: nat)
+  (u: uinttype t n)
+  (len: U32.t)
+  (x0: t)
+  (y: U32.t * t * B32.bytes)
+: Pure (bool * (U32.t * t * B32.bytes))
+  (requires (n_to_be_inv t n u len x0 true y))
+  (ensures (fun (continue, y') ->
+    n_to_be_inv t n u len x0 continue y' /\
+    (continue == true ==> n_to_be_measure t y' < n_to_be_measure t y)
+  ))
+= let (i, x, accu) = y in
+  if i = 0ul
+  then (false, y)
+  else
+    let accu' = n_to_be_body' t n u x0 i x accu in
+    let x' = u.div256 x in
+    let i' = U32.sub i 1ul in
+    (true, (i', x', accu'))
+
+inline_for_extraction
+let n_to_be_impl
+  (t: Type0)
+  (n: nat)
+  (u: uinttype t n)
+  (len: U32.t)
+  (x0: t)
+  (z: unit {
+    u.v x0 < pow2 (8 `Prims.op_Multiply` U32.v len) /\
+    8 `Prims.op_Multiply` U32.v len <= n
+  } )
+: Tot (y: B32.bytes { B32.reveal y == n_to_be len (u.v x0) } )
+= let buf = B32.create len 42uy in
+  Seq.append_empty_r (n_to_be len (u.v x0));
+  let (_, _, res) =
+    CL.total_while
+      (n_to_be_measure t)
+      (n_to_be_inv t n u len x0)
+      (n_to_be_body t n u len x0)
+      (len, x0, buf)
+  in
+  Seq.append_empty_l (B32.reveal res);
+  res
+
+
+module U16 = FStar.UInt16
+module U32 = FStar.UInt32
+module Cast = FStar.Int.Cast
+
+inline_for_extraction
+let u8 : uinttype U8.t 8 =
+  UIntType
+    (fun x -> U8.v x)
+    (fun x -> x)
+    (fun x -> x)
+    0uy
+    (fun x y -> ())
+    (fun x y -> U8.add x y)
+    (fun x -> 0uy)
+    (fun x -> 0uy)
+
+inline_for_extraction
+let u16 : uinttype U16.t 16 =
+  UIntType
+    (fun x -> U16.v x)
+    (fun x -> Cast.uint16_to_uint8 x)
+    (fun x -> Cast.uint8_to_uint16 x)
+    0us
+    (fun x y -> ())
+    (fun x y -> U16.add x y)
+    (fun x -> U16.mul x 256us)
+    (fun x -> U16.div x 256us)
+
+inline_for_extraction
+let u32 : uinttype U32.t 32 =
+  UIntType
+    (fun x -> U32.v x)
+    (fun x -> Cast.uint32_to_uint8 x)
+    (fun x -> Cast.uint8_to_uint32 x)
+    0ul
+    (fun x y -> ())
+    (fun x y -> U32.add x y)
+    (fun x -> U32.mul x 256ul)
+    (fun x -> U32.div x 256ul)
